

Backward Substitution:

In forward substitution, put $n = 0, 1, 2, \dots$ in the given recurrence relation until, a pattern is seen.

In backward substitution, do the reverse $n = n, n-1, n-2, \dots$ or $n = n, n/2, n/4, \dots$ until a pattern is seen.

After a pattern is seen, make a guess

Consider the recurrence relation:

$$T(n) = \begin{cases} 1, & \text{if } n=1 \\ 2T\left(\frac{n}{2}\right) + n, & \text{otherwise} \end{cases} \quad \text{--- (1)}$$

Given $T(n)$, find $T\left(\frac{n}{2}\right)$ in (1)

$$T\left(\frac{n}{2}\right) = 2T\left(\frac{\frac{n}{2}}{2}\right) + \frac{n}{2} = 2T\left(\frac{n}{4}\right) + \frac{n}{2}$$

back substitute value of $T\left(\frac{n}{2}\right)$ in $T(n)$ (1)

$$T(n) = 2^2 T\left(\frac{n}{2^2}\right) + 2n$$

Similarly, $T(n) = 2^3 T\left(\frac{n}{2^3}\right) + 3n$

$$= 2^4 T\left(\frac{n}{2^4}\right) + 4n$$

$$= 2^k T\left(\frac{n}{2^k}\right) + kn$$

Apply boundary condition i.e., $T(1) = 1$

$$\therefore \text{for } T(1) = 1, \frac{n}{2^k} = 1 \quad \text{--- (2)}$$

Taking \log_2 on both sides

$$n = \log_2 n$$

the equation becomes

$$T(n) = 2^{\log_2 n} T\left(\frac{n}{2^{\log_2 n}}\right) + \log_2 n \cdot n$$

$$= n T(1) + n \log_2 n$$

$$= n \log_2 n + n$$

The correctness is verified using induction,
 $n = 2, 4, 8, 16, \dots$

✓
Verified $T(2) = 2 \log_2 2 + 2$
 $= 2(1) + 2 = 4$

✗
Not applicable $T(3) = 3 \log_2 3 + 3$

✓
Verified $T(4) = 4 \log_2 4 + 4$
 $= 4 \log_2 2^2 + 4$
 $= 8 \log_2 2 + 4$
 $= 8 + 4 = 12$

Given

$$T(n) = 2T\left(\frac{n}{2}\right) + n$$

$$T(2) = 2T(1) + 2$$
$$= 2(1) + 2$$
$$= 4$$

✗
 $T(3) = 2T\left(\frac{3}{2}\right) + 3$

✓
 $T(4) = 2T\left(\frac{4}{2}\right) + 4$

$$T(4) = 2T\left(\frac{4}{2}\right) + 4$$

$$T(4) = 2T(2) + 4$$
$$= 2(4) + 4$$
$$= 8 + 4 = 12$$

Solving Recurrence Relations: Substitution Forward Substitution Method:

Step 1: Solve the recurrence relation for $n = 0, 1, 2, \dots$ until a pattern is obtained.

Step 2: Make a guess and predict the running time.

Step 3: Verify the guess work using induction.

Consider the recurrence relation:

$$T(n) = \begin{cases} 1 & \text{if } n=1 \\ T(n-1) + 1, & \text{otherwise} \end{cases}$$

Calculate the running time for $n=0, 1, 2$

$$n \quad T(n)$$

$$1 \quad T(1-1) + 1 = T(0) + 1$$

as defined in $T(n)$, $T(n)=1$, if $n=1$

$$2 \quad T(2-1) + 1 = 1 + 1 = 2$$

$$3 \quad T(3-1) + 1 = 1 + 1 + 1 = 3$$

$$4 \quad T(4-1) + 1 = 1 + 1 + 1 + 1 = 4$$

\therefore when $n=k$, $T(n)=k$,

Hence, running time is

$$\boxed{T(n) = n}$$

To Verify by Induction,

$$T(n) = n, T(1) = 1, T(2) = 2, T(3) = 3, \dots$$

Example: 2

$$T(n) = \begin{cases} 1, & \text{if } n=1 \\ 2T(n-1)+1, & \text{otherwise} \end{cases}$$

$n \quad T(n)$

$$1 \quad 1$$

$$2 \quad 2.T(2-1)+1 = 2.1+1 = 3$$

$$3 \quad 2.T(3-1)+1 = 2.2.1+2.1+1 = 7$$

$$4 \quad 2.T(4-1)+1 = 2.2.2.1 + 2.2.1 + 2.1 + 1 = 15$$

$$5 \quad 2.T(5-1)+1 = 2.2.2.2.1 + 2.2.2.1 + 2.2.1 + 2.1 + 1 = 31$$

To see a pattern, when value of n is k

$$T(k) = 2^{k-1} + 2^{k-2} + \dots + 2^0$$

This is a geometric series, $\left[\begin{array}{l} \text{*Refer to} \\ \text{Lecture material} \\ \text{Asymptotic Notation} \\ \text{Review on Summation} \\ \text{and functions} \end{array} \right]$
Sum is calculated as

$$2^k - 1$$

The running time of algorithm is

$$T(n) = 2^n - 1$$

①

The correctness of this running time can be verified for $n=1, 2, 3$ in ①